backend/Linearizeproof.v
@@ -704,6 +704,23 @@ Proof.
   econstructor; eauto.
 Qed.
 
+Lemma transf_entry_points:
+   forall (s1 : LTL.state) (f : val) (arg : list val) (m0 : mem),
+  LTL.entry_point prog m0 s1 f arg ->
+  exists s2 : Linear.state, Linear.entry_point tprog m0 s2 f arg /\ match_states s1 s2.
+Proof.
+  intros. inv H. subst ge0.
+  exploit function_ptr_translated; eauto. intros (tf & A & B).
+  econstructor; split.
+  - econstructor; eauto.
+    eapply globals_not_fresh_preserve; simpl in *; try eassumption.
+      eapply match_program_gen_len_defs in TRANSF; eauto.
+    erewrite sig_preserved; eauto.
+  - erewrite sig_preserved by eauto.
+    econstructor; eauto.
+    constructor.
+Qed.
+
 Lemma transf_initial_states:
   forall st1, LTL.initial_state prog st1 ->
   exists st2, Linear.initial_state tprog st2 /\ match_states st1 st2.
@@ -730,6 +747,7 @@ Theorem transf_program_correct:
 Proof.
   eapply forward_simulation_star.
   apply senv_preserved.
+  eexact transf_entry_points.
   eexact transf_initial_states.
   eexact transf_final_states.
   eexact transf_step_correct.
